another refactor in the books

dependency_test/b.py
@@ -1,4 +1,0 @@
-from dependency_test.c import c
-
-def b():
-    return "b" + c()
