python/Demo2x.py
@@ -1,7 +1,0 @@
-import M
-
-def main():
-    print("Hi");
-    M.C.p();
-
-main()
