python/demo2/Demo2x.py
@@ -1,9 +1,0 @@
-import sys
-sys.path.append('Demo2-py')
-import M
-
-def main():
-    print("Hi")
-    M.C.p()
-
-main()
