formic_site_duct/implementations/login_challenge.program.dfy
@@ -1,4 +1,4 @@
-module DuctUserInfoImpl {
+module DuctLoginImpl {
 
   import opened DB
   import opened DuctTools
@@ -8,8 +8,34 @@ module DuctUserInfoImpl {
 
     constructor () {}
 
-    function Implementation(u: UserInfo): GeneratedEndpointResult
+    function Implementation(u: UserInfo, before: seq<DbValue>): GeneratedEndpointResult
     {
+      GeneratedEndpointResult(Return, ChallengeGoogle("/save_user"))
+    }
+
+    lemma ProveImplementationCorrect(u: UserInfo)
+      requires PreCondition(u)
+      ensures ImplementationCorrect(u)
+    {
+      assert forall before: seq<DbValue> ::
+        PostCondition(
+          u,
+          before,
+          Implementation(u, before).response,
+          ExecuteProgram(before, Implementation(u, before).program)) by {
+        forall before: seq<DbValue>
+          ensures PostCondition(
+            u,
+            before,
+            Implementation(u, before).response,
+            ExecuteProgram(before, Implementation(u, before).program))
+        {
+          assert Implementation(u, before).response == ChallengeGoogle("/save_user");
+          assert Implementation(u, before).program == Return;
+          assert ProgramOperations(before, Implementation(u, before).program) == [];
+          assert ExecuteProgram(before, Implementation(u, before).program) == before;
+        }
+      }
     }
   }
 }
