formic_site_duct/implementations/user_info.program.dfy
@@ -1,4 +1,4 @@
-module DuctSaveUserImpl {
+module DuctUserInfoImpl {
 
   import opened DB
   import opened DuctTools
@@ -8,15 +8,34 @@ module DuctSaveUserImpl {
 
     constructor () {}
 
-    function Implementation(u: UserInfo): GeneratedEndpointResult
+    function Implementation(u: UserInfo, before: seq<DbValue>): GeneratedEndpointResult
     {
-        
+      GeneratedEndpointResult(Return, Content(NatToString(|before|)))
     }
 
     lemma ProveImplementationCorrect(u: UserInfo)
       requires PreCondition(u)
       ensures ImplementationCorrect(u)
     {
+      assert forall before: seq<DbValue> ::
+        PostCondition(
+          u,
+          before,
+          Implementation(u, before).response,
+          ExecuteProgram(before, Implementation(u, before).program)) by {
+        forall before: seq<DbValue>
+          ensures PostCondition(
+            u,
+            before,
+            Implementation(u, before).response,
+            ExecuteProgram(before, Implementation(u, before).program))
+        {
+          assert Implementation(u, before).response == Content(NatToString(|before|));
+          assert Implementation(u, before).program == Return;
+          assert ProgramOperations(before, Implementation(u, before).program) == [];
+          assert ExecuteProgram(before, Implementation(u, before).program) == before;
+        }
+      }
     }
   }
 }
