dafny_test/Demo1.dfy
@@ -1,6 +1,0 @@
-module M {
-  method {:extern "Demo", "p"} p() 
-  method Main() {
-    p();
-  }
-}
